feat: Q is a field

LeanMath/Basic.lean
@@ -42,3 +42,30 @@ example : Q.mk (Z.mk (1, 0), two) + Q.mk (Z.mk (2, 0), four) = Q.mk (two, two) :
   simp only [OfNat.ofNat, ofNat, N.mul_zero, N.zero_mul, N.add_zero, N.zero_add]
   simp only [HMul.hMul, Mul.mul, N.mul]
   simp only [N.add_comm, N.add_succ, N.add_zero, Z.eqv_is_refl]
+
+def coeN : N -> Nat
+  | N.zero => Nat.zero
+  | N.succ n => Nat.succ $ coeN n
+instance : Coe N Nat where
+  coe := coeN
+
+def coeN₂ (a : N × N) : Int := coeN a.fst - coeN a.snd
+theorem coeN₂_is_well_defined (a b : N × N) (h : Z.eqv a b) : coeN₂ a = coeN₂ b := sorry
+def coeZ : Z -> Int := Quotient.lift coeN₂ coeN₂_is_well_defined
+
+def coeZ₂ (a : Z₂) : Rat := coeZ a.fst / coeZ a.snd
+theorem coeZ₂_is_well_defined (a b : Z₂) (h : Q.eqv a b) : coeZ₂ a = coeZ₂ b := sorry
+def coeQ : Q -> Rat := Quotient.lift coeZ₂ coeZ₂_is_well_defined
+instance : Coe Q Rat where
+  coe := coeQ
+
+instance : ToString Q where
+  toString a := ToString.toString $ (Coe.coe a : Rat)
+
+#eval! coeQ $ Q.inv $ Q.mk (Z.one + Z.one, Q.nonZeroOne)
+#eval! Q.one
+
+#eval! Q.invZ₂ (Z.one + Z.one, Q.nonZeroOne)
+#eval! Q.invZ₂ (Z.zero, Q.nonZeroOne)
+#eval! Q.inv $ Q.mk (Z.one + Z.one, Q.nonZeroOne)
+#eval! Q.inv $ Q.mk (Z.zero, Q.nonZeroOne)
